Prove wellformedness, CT0, CT1 and CT2 for hiding

CTockTick_Hiding.thy
@@ -8,16 +8,334 @@ fun hide_trace :: "'a cttevent set \<Rightarrow> 'a cttobs list \<Rightarrow> 'a
   "hide_trace X [] = {[]}" |
   "hide_trace X ([Event e]\<^sub>E # s) =
     {t. (Event e \<in> X \<and> t \<in> hide_trace X s) \<or> (\<exists>s'. Event e \<notin> X \<and> s' \<in> hide_trace X s \<and> t = [Event e]\<^sub>E # s')}" |
-  "hide_trace X ([Tick]\<^sub>E # s) =
-    {t. (Tick \<in> X \<and> t \<in> hide_trace X s) \<or> (\<exists>s'. Tick \<notin> X \<and> s \<in> hide_trace X s \<and> t = [Tick]\<^sub>E # s')}" |
+  "hide_trace X ([[Tick]\<^sub>E]) =
+    {t. (Tick \<in> X \<and> t = []) \<or> (Tick \<notin> X \<and> t = [[Tick]\<^sub>E])}" |
   "hide_trace X ([Y]\<^sub>R # [Tock]\<^sub>E # s) =
-    {t. (Tock \<in> X \<and> t \<in> hide_trace X s) \<or> (\<exists> s'. \<exists> Z\<subseteq>X. Tock \<notin> X \<and> t = [Y \<union> Z]\<^sub>R # [Tock]\<^sub>E # s' \<and> s' \<in> hide_trace X s)}" |
-  "hide_trace X [[Y]\<^sub>R] = {t. \<exists> Z\<subseteq>X. t = [[Y \<union> Z]\<^sub>R]}" |
+    {t. (Tock \<in> X \<and> t \<in> hide_trace X s)
+    \<or> (\<exists> s'. \<exists> Z\<subseteq>Y. Tock \<notin> X \<and> X \<subseteq> Y \<and> t = [Z]\<^sub>R # [Tock]\<^sub>E # s' \<and> s' \<in> hide_trace X s)}" | (* fill in subsets to account for removed sets *)
+    (* if X \<subseteq> Y is not true an event in X could happen so the hidden event takes priority over tock *)
+  "hide_trace X [[Y]\<^sub>R] = {t. \<exists> Z\<subseteq>Y. X \<subseteq> Y \<and> t = [[Z]\<^sub>R]}" | (* fill in subsets to account for removed sets *)
+    (* if X \<subseteq> Y is not true an event in X could happen so instability is introduced when it is hidden *)
   "hide_trace X ([Tock]\<^sub>E # t) = {}" |
   "hide_trace X ([Y]\<^sub>R # [Event e]\<^sub>E # t) = {}" |
   "hide_trace X ([Y]\<^sub>R # [Tick]\<^sub>E # t) = {}" |
-  "hide_trace X ([Y]\<^sub>R # [Z]\<^sub>R # t) = {}"
+  "hide_trace X ([Y]\<^sub>R # [Z]\<^sub>R # t) = {}" |
+  "hide_trace X ([Tick]\<^sub>E # x # t) = {}"
 
 definition HidingCTT :: "'a cttobs list set \<Rightarrow> 'a cttevent set \<Rightarrow> 'a cttobs list set" (infixl "\<setminus>\<^sub>C" 53) where
   "HidingCTT P X = \<Union> {hide_trace X p | p. p \<in> P}"
 
+lemma HidingCTT_wf:
+  assumes "\<forall>x\<in>P. cttWF x"
+  shows "\<forall>x\<in>(P \<setminus>\<^sub>C X). cttWF x"
+  using assms unfolding HidingCTT_def
+proof auto
+  fix x p
+  show "\<And> P x. \<forall>x\<in>P. cttWF x \<Longrightarrow> x \<in> hide_trace X p \<Longrightarrow> p \<in> P \<Longrightarrow> cttWF x"
+    apply (induct p rule:hide_trace.induct, simp_all)
+    apply (metis cttWF.simps(4) mem_Collect_eq)
+    using cttWF.simps(1) apply blast
+    apply (metis cttWF.simps(5) mem_Collect_eq)
+    using cttWF.simps(2) by blast
+qed
+
+lemma CT0_Hiding:
+  assumes "CT0 P" "CT1 P"  
+  shows "CT0 (P \<setminus>\<^sub>C X)"
+  unfolding HidingCTT_def CT0_def
+proof auto
+  have "[] \<in> P"
+    by (simp add: CT0_CT1_empty assms(1) assms(2))
+  then show "\<exists>x. (\<exists>p. x = hide_trace X p \<and> p \<in> P) \<and> x \<noteq> {}"
+    using hide_trace.simps(1) by blast
+qed
+
+lemma CT1_Hiding:
+  shows "CT1 P \<Longrightarrow> CT1 (P \<setminus>\<^sub>C X)"
+  unfolding HidingCTT_def CT1_def
+proof auto
+  fix p
+  show "\<And>P \<rho> \<sigma>. \<forall>\<rho>. (\<exists>\<sigma>. \<rho> \<lesssim>\<^sub>C \<sigma> \<and> \<sigma> \<in> P) \<longrightarrow> \<rho> \<in> P \<Longrightarrow> \<rho> \<lesssim>\<^sub>C \<sigma> \<Longrightarrow> \<sigma> \<in> hide_trace X p \<Longrightarrow> p \<in> P \<Longrightarrow> \<exists>x. (\<exists>p. x = hide_trace X p \<and> p \<in> P) \<and> \<rho> \<in> x"
+  proof (induct p rule:hide_trace.induct, simp_all, safe, simp_all)
+    fix X :: "'a cttevent set"
+    fix \<rho> :: "'a cttobs list"
+    fix P :: "'a cttobs list set" 
+    assume case_assms: "\<rho> \<lesssim>\<^sub>C []" "[] \<in> P"
+    then have "\<rho> = []"
+      by (induct \<rho>, auto)
+    then show "\<exists>x. (\<exists>p. x = hide_trace X p \<and> p \<in> P) \<and> \<rho> \<in> x"
+      using case_assms by auto
+  next
+    fix X e s P \<rho> \<sigma>
+    assume ind_hyp: "\<And>P \<rho> \<sigma>. \<forall>\<rho>. (\<exists>\<sigma>. \<rho> \<lesssim>\<^sub>C \<sigma> \<and> \<sigma> \<in> P) \<longrightarrow> \<rho> \<in> P \<Longrightarrow>
+                 \<rho> \<lesssim>\<^sub>C \<sigma> \<Longrightarrow> \<sigma> \<in> hide_trace X s \<Longrightarrow> s \<in> P \<Longrightarrow> \<exists>x. (\<exists>p. x = hide_trace X p \<and> p \<in> P) \<and> \<rho> \<in> x"
+    assume case_assms: "\<forall>\<rho>. (\<exists>\<sigma>. \<rho> \<lesssim>\<^sub>C \<sigma> \<and> \<sigma> \<in> P) \<longrightarrow> \<rho> \<in> P" "\<rho> \<lesssim>\<^sub>C \<sigma>" "[Event e]\<^sub>E # s \<in> P" "Event e \<in> X" "\<sigma> \<in> hide_trace X s"
+    have 1: "\<forall>\<rho>. (\<exists>\<sigma>. \<rho> \<lesssim>\<^sub>C \<sigma> \<and> \<sigma> \<in> {t. [Event e]\<^sub>E # t \<in> P}) \<longrightarrow> \<rho> \<in> {t. [Event e]\<^sub>E # t \<in> P}"
+      using case_assms(1) ctt_prefix_subset.simps(3) by blast
+    have 2: "s \<in> {t. [Event e]\<^sub>E # t \<in> P}"
+      using case_assms by auto
+    obtain x p  where "x = hide_trace X p \<and> p \<in> {t. [Event e]\<^sub>E # t \<in> P} \<and> \<rho> \<in> x"
+      using 1 2 case_assms ind_hyp[where P="{t. [Event e]\<^sub>E # t \<in> P}", where \<rho>=\<rho>, where \<sigma>=\<sigma>] by blast
+    then show "\<exists>x. (\<exists>p. x = hide_trace X p \<and> p \<in> P) \<and> \<rho> \<in> x"
+      apply (rule_tac x="hide_trace X ([Event e]\<^sub>E # p)" in exI)
+      by (metis (no_types, lifting) case_assms(4) hide_trace.simps(2) mem_Collect_eq)
+  next
+    fix X e s P \<rho> s'
+    assume ind_hyp: "\<And>P \<rho> \<sigma>. \<forall>\<rho>. (\<exists>\<sigma>. \<rho> \<lesssim>\<^sub>C \<sigma> \<and> \<sigma> \<in> P) \<longrightarrow> \<rho> \<in> P \<Longrightarrow>
+                 \<rho> \<lesssim>\<^sub>C \<sigma> \<Longrightarrow> \<sigma> \<in> hide_trace X s \<Longrightarrow> s \<in> P \<Longrightarrow> \<exists>x. (\<exists>p. x = hide_trace X p \<and> p \<in> P) \<and> \<rho> \<in> x"
+    assume case_assms: "\<forall>\<rho>. (\<exists>\<sigma>. \<rho> \<lesssim>\<^sub>C \<sigma> \<and> \<sigma> \<in> P) \<longrightarrow> \<rho> \<in> P" "\<rho> \<lesssim>\<^sub>C [Event e]\<^sub>E # s'"
+      "[Event e]\<^sub>E # s \<in> P" "Event e \<notin> X" "s' \<in> hide_trace X s"
+    have "(\<exists>\<rho>'. \<rho>' \<lesssim>\<^sub>C s' \<and> \<rho> = [Event e]\<^sub>E # \<rho>') \<or> \<rho> = []"
+      using case_assms(2) by (cases \<rho>, auto, (case_tac a, auto)+)
+    then show "\<exists>x. (\<exists>p. x = hide_trace X p \<and> p \<in> P) \<and> \<rho> \<in> x"
+    proof auto
+      fix \<rho>'
+      assume case_assms2: "\<rho>' \<lesssim>\<^sub>C s'" "\<rho> = [Event e]\<^sub>E # \<rho>'"
+      have 1: "\<forall>\<rho>. (\<exists>\<sigma>. \<rho> \<lesssim>\<^sub>C \<sigma> \<and> \<sigma> \<in> {t. [Event e]\<^sub>E # t \<in> P}) \<longrightarrow> \<rho> \<in> {t. [Event e]\<^sub>E # t \<in> P}"
+        using case_assms(1) ctt_prefix_subset.simps(3) by blast
+      have 2: "s \<in> {t. [Event e]\<^sub>E # t \<in> P}"
+        by (simp add: case_assms(3))
+      obtain x p where "x = hide_trace X p \<and> p \<in> {t. [Event e]\<^sub>E # t \<in> P} \<and> \<rho>' \<in> x"
+        using ind_hyp[where P="{t. [Event e]\<^sub>E # t \<in> P}", where \<rho>=\<rho>', where \<sigma>=s'] 1 2 case_assms2 case_assms(5) by blast
+      then show "\<exists>x. (\<exists>p. x = hide_trace X p \<and> p \<in> P) \<and> [Event e]\<^sub>E # \<rho>' \<in> x"
+        by (rule_tac x="hide_trace X ([Event e]\<^sub>E # p)" in exI, auto, rule_tac x="[Event e]\<^sub>E # p" in exI, auto simp add: case_assms)
+    next
+      show "\<rho> = [] \<Longrightarrow> \<exists>x. (\<exists>p. x = hide_trace X p \<and> p \<in> P) \<and> [] \<in> x"
+        apply (rule_tac x="hide_trace X []" in exI, auto, rule_tac x="[]" in exI, auto)
+        using case_assms(1) case_assms(3) ctt_prefix_subset.simps(1) by blast
+    qed
+  next
+    fix X :: "'a cttevent set"
+    fix \<rho> :: "'a cttobs list"
+    fix P :: "'a cttobs list set" 
+    assume case_assms: "\<rho> \<lesssim>\<^sub>C []" "[[Tick]\<^sub>E] \<in> P" "\<forall>\<rho>. (\<exists>\<sigma>. \<rho> \<lesssim>\<^sub>C \<sigma> \<and> \<sigma> \<in> P) \<longrightarrow> \<rho> \<in> P"
+    then have "\<rho> = []"
+      by (cases \<rho>, auto)
+    then show "\<exists>x. (\<exists>p. x = hide_trace X p \<and> p \<in> P) \<and> \<rho> \<in> x"
+      apply (rule_tac x="hide_trace X []" in exI, auto, rule_tac x="[]" in exI, auto)
+      using case_assms(2) case_assms(3) ctt_prefix_subset.simps(1) by blast
+  next
+    fix X :: "'a cttevent set"
+    fix \<rho> :: "'a cttobs list"
+    fix P :: "'a cttobs list set" 
+    assume case_assms: "\<forall>\<rho>. (\<exists>\<sigma>. \<rho> \<lesssim>\<^sub>C \<sigma> \<and> \<sigma> \<in> P) \<longrightarrow> \<rho> \<in> P" "\<rho> \<lesssim>\<^sub>C [[Tick]\<^sub>E]" "[[Tick]\<^sub>E] \<in> P" "Tick \<notin> X"
+    then have "\<rho> = [] \<or> \<rho> = [[Tick]\<^sub>E]"
+      by (cases \<rho>, simp, case_tac a, simp_all, case_tac list, simp_all)
+    then show "\<exists>x. (\<exists>p. x = hide_trace X p \<and> p \<in> P) \<and> \<rho> \<in> x"
+      apply (auto, rule_tac x="hide_trace X []" in exI, auto, rule_tac x="[]" in exI, auto)
+      using case_assms ctt_prefix_subset.simps(1) by (blast, auto)
+  next
+    fix X Y s P \<rho> \<sigma>
+    assume ind_hyp: "\<And>P \<rho> \<sigma>. \<forall>\<rho>. (\<exists>\<sigma>. \<rho> \<lesssim>\<^sub>C \<sigma> \<and> \<sigma> \<in> P) \<longrightarrow> \<rho> \<in> P \<Longrightarrow>
+                 \<rho> \<lesssim>\<^sub>C \<sigma> \<Longrightarrow> \<sigma> \<in> hide_trace X s \<Longrightarrow> s \<in> P \<Longrightarrow> \<exists>x. (\<exists>p. x = hide_trace X p \<and> p \<in> P) \<and> \<rho> \<in> x"
+    assume case_assms: "\<forall>\<rho>. (\<exists>\<sigma>. \<rho> \<lesssim>\<^sub>C \<sigma> \<and> \<sigma> \<in> P) \<longrightarrow> \<rho> \<in> P" "\<rho> \<lesssim>\<^sub>C \<sigma>" "[Y]\<^sub>R # [Tock]\<^sub>E # s \<in> P" "Tock \<in> X" "\<sigma> \<in> hide_trace X s"
+    have 1: "\<forall>\<rho>. (\<exists>\<sigma>. \<rho> \<lesssim>\<^sub>C \<sigma> \<and> \<sigma> \<in> {t. [Y]\<^sub>R # [Tock]\<^sub>E # t \<in> P}) \<longrightarrow> \<rho> \<in> {t. [Y]\<^sub>R # [Tock]\<^sub>E # t \<in> P}"
+      by (metis case_assms(1) ctt_prefix_subset.simps(2) ctt_prefix_subset.simps(3) ctt_subset.simps(2) ctt_subset_refl mem_Collect_eq)
+    have 2: "s \<in> {t. [Y]\<^sub>R # [Tock]\<^sub>E # t \<in> P}"
+      by (simp add: case_assms(3))
+    obtain x p where "x = hide_trace X p \<and> p \<in> {t. [Y]\<^sub>R # [Tock]\<^sub>E # t \<in> P} \<and> \<rho> \<in> x"
+      using ind_hyp[where P="{t. [Y]\<^sub>R # [Tock]\<^sub>E # t \<in> P}", where \<rho>=\<rho>, where \<sigma>=\<sigma>] 1 2 case_assms by blast
+    then show "\<exists>x. (\<exists>p. x = hide_trace X p \<and> p \<in> P) \<and> \<rho> \<in> x"
+      apply (rule_tac x="hide_trace X ([Y]\<^sub>R # [Tock]\<^sub>E # p)" in exI, auto)
+      by (rule_tac x="[Y]\<^sub>R # [Tock]\<^sub>E # p" in exI, auto simp add: case_assms(4))
+  next
+    fix X Y s P \<rho> s' Z
+    assume ind_hyp: "\<And>P \<rho> \<sigma>. \<forall>\<rho>. (\<exists>\<sigma>. \<rho> \<lesssim>\<^sub>C \<sigma> \<and> \<sigma> \<in> P) \<longrightarrow> \<rho> \<in> P \<Longrightarrow>
+                 \<rho> \<lesssim>\<^sub>C \<sigma> \<Longrightarrow> \<sigma> \<in> hide_trace X s \<Longrightarrow> s \<in> P \<Longrightarrow> \<exists>x. (\<exists>p. x = hide_trace X p \<and> p \<in> P) \<and> \<rho> \<in> x"
+    assume case_assms: "\<forall>\<rho>. (\<exists>\<sigma>. \<rho> \<lesssim>\<^sub>C \<sigma> \<and> \<sigma> \<in> P) \<longrightarrow> \<rho> \<in> P" "\<rho> \<lesssim>\<^sub>C [Z]\<^sub>R # [Tock]\<^sub>E # s'"
+      "[Y]\<^sub>R # [Tock]\<^sub>E # s \<in> P" "Z \<subseteq> Y" "Tock \<notin> X" "X \<subseteq> Y" "s' \<in> hide_trace X s"
+    have 1: "\<forall>\<rho>. (\<exists>\<sigma>. \<rho> \<lesssim>\<^sub>C \<sigma> \<and> \<sigma> \<in> {t. [Y]\<^sub>R # [Tock]\<^sub>E # t \<in> P}) \<longrightarrow> \<rho> \<in> {t. [Y]\<^sub>R # [Tock]\<^sub>E # t \<in> P}"
+      by (metis case_assms(1) ctt_prefix_subset.simps(2) ctt_prefix_subset.simps(3) mem_Collect_eq subset_refl)
+    have 2: "s \<in> {t. [Y]\<^sub>R # [Tock]\<^sub>E # t \<in> P}"
+      by (simp add: case_assms(3))
+    have "(\<exists> \<rho>' W. \<rho> = [W]\<^sub>R # [Tock]\<^sub>E # \<rho>' \<and> W \<subseteq> Z) \<or> (\<exists> W. \<rho> = [[W]\<^sub>R] \<and> W \<subseteq> Z) \<or> (\<rho> = [])"
+      using case_assms(2) by (cases \<rho> rule:cttWF.cases, simp_all)
+    then show "\<exists>x. (\<exists>p. x = hide_trace X p \<and> p \<in> P) \<and> \<rho> \<in> x"
+    proof auto
+      fix \<rho>' W
+      assume case_assms2: "W \<subseteq> Z" "\<rho> = [W]\<^sub>R # [Tock]\<^sub>E # \<rho>'"
+      have "\<rho>' \<lesssim>\<^sub>C s'"
+        using case_assms(2) case_assms2(2) by auto
+      then obtain x p where "x = hide_trace X p \<and> p \<in> {t. [Y]\<^sub>R # [Tock]\<^sub>E # t \<in> P} \<and> \<rho>' \<in> x"
+        using ind_hyp[where P="{t. [Y]\<^sub>R # [Tock]\<^sub>E # t \<in> P}", where \<rho>=\<rho>', where \<sigma>=s'] 1 2 case_assms(7) by blast 
+      then show "\<exists>x. (\<exists>p. x = hide_trace X p \<and> p \<in> P) \<and> [W]\<^sub>R # [Tock]\<^sub>E # \<rho>' \<in> x"
+        apply (rule_tac x="hide_trace X ([Y]\<^sub>R # [Tock]\<^sub>E # p)" in exI, safe)
+        using case_assms2(1) case_assms(4) case_assms(5) case_assms(6) by (rule_tac x="[Y]\<^sub>R # [Tock]\<^sub>E # p" in exI, auto)
+    next
+      fix W
+      assume case_assms2: "W \<subseteq> Z" "\<rho> = [[W]\<^sub>R]"
+      then show "\<exists>x. (\<exists>p. x = hide_trace X p \<and> p \<in> P) \<and> [[W]\<^sub>R] \<in> x"
+        apply (rule_tac x="hide_trace X ([[Y]\<^sub>R])" in exI, safe)
+        using case_assms(4) case_assms(5) case_assms(6) apply (rule_tac x="[[Y]\<^sub>R]" in exI, auto)
+        using case_assms(1) case_assms(3) ctt_prefix_subset.simps(1) ctt_prefix_subset.simps(2) by blast
+    next
+      show "\<rho> = [] \<Longrightarrow> \<exists>x. (\<exists>p. x = hide_trace X p \<and> p \<in> P) \<and> [] \<in> x"
+        using case_assms(1) case_assms(3) ctt_prefix_subset.simps(1) hide_trace.simps(1) by blast
+    qed
+  next
+    fix X Y P \<rho> Z
+    assume case_assms: "\<forall>\<rho>. (\<exists>\<sigma>. \<rho> \<lesssim>\<^sub>C \<sigma> \<and> \<sigma> \<in> P) \<longrightarrow> \<rho> \<in> P" "\<rho> \<lesssim>\<^sub>C [[Z]\<^sub>R]" "[[Y]\<^sub>R] \<in> P" "Z \<subseteq> Y" "X \<subseteq> Y "
+    then have "(\<exists> W. \<rho> = [[W]\<^sub>R] \<and> W \<subseteq> Z) \<or> (\<rho> = [])"
+      using case_assms(2) by (cases \<rho> rule:cttWF.cases, simp_all)
+    then show "\<exists>x. (\<exists>p. x = hide_trace X p \<and> p \<in> P) \<and> \<rho> \<in> x"
+      apply auto apply (rule_tac x="hide_trace X ([[Y]\<^sub>R])" in exI, safe)
+      using case_assms apply (rule_tac x="[[Y]\<^sub>R]" in exI, auto)
+      apply (rule_tac x="{[]}" in exI, simp, rule_tac x="[]" in exI, simp)
+      using ctt_prefix_subset.simps(1) by blast
+  qed
+qed
+
+lemma CT2_Hiding:
+  assumes "CT2 P"
+  shows "CT2 (P \<setminus>\<^sub>C X)"
+  unfolding CT2_def HidingCTT_def
+proof auto
+  fix Xa Y p
+  show "\<And> \<rho>. Y \<inter> {e. e \<noteq> Tock \<and> (\<exists>x. (\<exists>p. x = hide_trace X p \<and> p \<in> P) \<and> \<rho> @ [[e]\<^sub>E] \<in> x) \<or>
+      e = Tock \<and> (\<exists>x. (\<exists>p. x = hide_trace X p \<and> p \<in> P) \<and> \<rho> @ [[Xa]\<^sub>R, [e]\<^sub>E] \<in> x)} = {} \<Longrightarrow>
+    \<rho> @ [[Xa]\<^sub>R] \<in> hide_trace X p \<Longrightarrow> p \<in> P \<Longrightarrow> \<exists>x. (\<exists>p. x = hide_trace X p \<and> p \<in> P) \<and> \<rho> @ [[Xa \<union> Y]\<^sub>R] \<in> x"
+    using assms
+  proof -
+    show "\<And>P \<rho>. Y \<inter> {e. e \<noteq> Tock \<and> (\<exists>x. (\<exists>p. x = hide_trace X p \<and> p \<in> P) \<and> \<rho> @ [[e]\<^sub>E] \<in> x) \<or>
+        e = Tock \<and> (\<exists>x. (\<exists>p. x = hide_trace X p \<and> p \<in> P) \<and> \<rho> @ [[Xa]\<^sub>R, [e]\<^sub>E] \<in> x)} = {} \<Longrightarrow>
+      \<rho> @ [[Xa]\<^sub>R] \<in> hide_trace X p \<Longrightarrow> p \<in> P \<Longrightarrow> CT2 P \<Longrightarrow> \<exists>x. (\<exists>p. x = hide_trace X p \<and> p \<in> P) \<and> \<rho> @ [[Xa \<union> Y]\<^sub>R] \<in> x"
+    proof (induct p rule:cttWF.induct, simp_all, safe, simp_all)
+      fix Xb P
+      assume case_assms: "Y \<inter> {e. e \<noteq> Tock \<and> (\<exists>x. (\<exists>p. x = hide_trace X p \<and> p \<in> P) \<and> [[e]\<^sub>E] \<in> x) \<or>
+                      e = Tock \<and> (\<exists>x. (\<exists>p. x = hide_trace X p \<and> p \<in> P) \<and> [[Xa]\<^sub>R, [e]\<^sub>E] \<in> x)} = {}"
+        "[[Xb]\<^sub>R] \<in> P" "CT2 P" "Xa \<subseteq> Xb" "X \<subseteq> Xb"
+      have "{e. e\<notin>X \<and> (e \<noteq> Tock \<and> [[e]\<^sub>E] \<in> P \<or> e = Tock \<and> [[Xb]\<^sub>R, [e]\<^sub>E] \<in> P)} \<subseteq>
+        {e. e \<noteq> Tock \<and> (\<exists>x. (\<exists>p. x = hide_trace X p \<and> p \<in> P) \<and> [[e]\<^sub>E] \<in> x) \<or>
+          e = Tock \<and> (\<exists>x. (\<exists>p. x = hide_trace X p \<and> p \<in> P) \<and> [[Xa]\<^sub>R, [e]\<^sub>E] \<in> x)}"
+      proof auto
+        fix x
+        show "x \<notin> X \<Longrightarrow> [[x]\<^sub>E] \<in> P \<Longrightarrow> x \<noteq> Tock \<Longrightarrow> \<exists>xa. (\<exists>p. xa = hide_trace X p \<and> p \<in> P) \<and> [[x]\<^sub>E] \<in> xa"
+          by (rule_tac x="hide_trace X [[x]\<^sub>E]" in exI, auto, cases x, auto)
+      next
+        fix x
+        show "x \<notin> X \<Longrightarrow> [[x]\<^sub>E] \<in> P \<Longrightarrow> x \<noteq> Tock \<Longrightarrow> \<exists>xa. (\<exists>p. xa = hide_trace X p \<and> p \<in> P) \<and> [[x]\<^sub>E] \<in> xa"
+          by (rule_tac x="hide_trace X [[x]\<^sub>E]" in exI, auto, cases x, auto)
+      next
+        show "Tock \<notin> X \<Longrightarrow> [[Xb]\<^sub>R, [Tock]\<^sub>E] \<in> P \<Longrightarrow> \<forall>x. (\<forall>p. x = hide_trace X p \<longrightarrow> p \<notin> P) \<or> [[Xa]\<^sub>R, [Tock]\<^sub>E] \<notin> x \<Longrightarrow> False"
+          using case_assms by (erule_tac x="hide_trace X [[Xb]\<^sub>R, [Tock]\<^sub>E]" in allE, auto)
+      next
+        show "Tock \<notin> X \<Longrightarrow> [[Xb]\<^sub>R, [Tock]\<^sub>E] \<in> P \<Longrightarrow> \<forall>x. (\<forall>p. x = hide_trace X p \<longrightarrow> p \<notin> P) \<or> [[Xa]\<^sub>R, [Tock]\<^sub>E] \<notin> x \<Longrightarrow> \<exists>x. (\<exists>p. x = hide_trace X p \<and> p \<in> P) \<and> [[Tock]\<^sub>E] \<in> x"
+          using case_assms by (erule_tac x="hide_trace X [[Xb]\<^sub>R, [Tock]\<^sub>E]" in allE, auto)
+      qed
+      then have "{x. x \<notin> X} \<inter> Y \<inter> {e. e\<notin>X \<and> (e \<noteq> Tock \<and> [[e]\<^sub>E] \<in> P \<or> e = Tock \<and> [[Xb]\<^sub>R, [e]\<^sub>E] \<in> P)} = {}"
+        using Int_empty_right case_assms(1) by auto
+      then have "[[Xb \<union> ({x. x \<notin> X} \<inter> Y)]\<^sub>R] \<in> P"
+        using case_assms unfolding CT2_def by (erule_tac x="[]" in allE, erule_tac x="Xb" in allE, erule_tac x="{x. x \<notin> X} \<inter> Y" in allE, auto)
+      also have "Xb \<union> ({x. x \<notin> X} \<inter> Y) = Xb \<union> Y"
+        using case_assms by auto
+      then have "[[Xb \<union> Y]\<^sub>R] \<in> P"
+        using calculation by auto
+      then show "\<exists>x. (\<exists>p. x = hide_trace X p \<and> p \<in> P) \<and> [[Xa \<union> Y]\<^sub>R] \<in> x"
+        using case_assms by (rule_tac x="hide_trace X [[Xb \<union> Y]\<^sub>R]" in exI, auto)
+    next
+      fix e \<sigma> P \<rho>
+      assume ind_hyp: "\<And>P \<rho>. Y \<inter> {e. e \<noteq> Tock \<and> (\<exists>x. (\<exists>p. x = hide_trace X p \<and> p \<in> P) \<and> \<rho> @ [[e]\<^sub>E] \<in> x) \<or>
+                       e = Tock \<and> (\<exists>x. (\<exists>p. x = hide_trace X p \<and> p \<in> P) \<and> \<rho> @ [[Xa]\<^sub>R, [e]\<^sub>E] \<in> x)} = {} \<Longrightarrow>
+        \<rho> @ [[Xa]\<^sub>R] \<in> hide_trace X \<sigma> \<Longrightarrow> \<sigma> \<in> P \<Longrightarrow> CT2 P \<Longrightarrow> \<exists>x. (\<exists>p. x = hide_trace X p \<and> p \<in> P) \<and> \<rho> @ [[Xa \<union> Y]\<^sub>R] \<in> x"
+      assume case_assms: "Y \<inter> {e. e \<noteq> Tock \<and> (\<exists>x. (\<exists>p. x = hide_trace X p \<and> p \<in> P) \<and> \<rho> @ [[e]\<^sub>E] \<in> x) \<or>
+                e = Tock \<and> (\<exists>x. (\<exists>p. x = hide_trace X p \<and> p \<in> P) \<and> \<rho> @ [[Xa]\<^sub>R, [e]\<^sub>E] \<in> x)} = {}"
+        "[Event e]\<^sub>E # \<sigma> \<in> P" "CT2 P" "Event e \<in> X" "\<rho> @ [[Xa]\<^sub>R] \<in> hide_trace X \<sigma>"
+      have "{ea. ea \<noteq> Tock \<and> (\<exists>x. (\<exists>p. x = hide_trace X p \<and> p \<in> {\<sigma>. [Event e]\<^sub>E # \<sigma> \<in> P}) \<and> \<rho> @ [[ea]\<^sub>E] \<in> x) \<or>
+              ea = Tock \<and> (\<exists>x. (\<exists>p. x = hide_trace X p \<and> p \<in> {\<sigma>. [Event e]\<^sub>E # \<sigma> \<in> P}) \<and> \<rho> @ [[Xa]\<^sub>R, [ea]\<^sub>E] \<in> x)} \<subseteq>
+        {e. e \<noteq> Tock \<and> (\<exists>x. (\<exists>p. x = hide_trace X p \<and> p \<in> P) \<and> \<rho> @ [[e]\<^sub>E] \<in> x) \<or>
+                e = Tock \<and> (\<exists>x. (\<exists>p. x = hide_trace X p \<and> p \<in> P) \<and> \<rho> @ [[Xa]\<^sub>R, [e]\<^sub>E] \<in> x)}"
+        using case_assms(4) apply (safe, simp_all)
+        apply (rule_tac x="hide_trace X ([Event e]\<^sub>E # p)" in exI, simp, rule_tac x="[Event e]\<^sub>E # p" in exI, simp)
+        apply (rule_tac x="hide_trace X ([Event e]\<^sub>E # p)" in exI, simp, rule_tac x="[Event e]\<^sub>E # p" in exI, simp)
+        apply (erule_tac x="hide_trace X ([Event e]\<^sub>E # p)" in allE, simp)
+        by (erule_tac x="hide_trace X ([Event e]\<^sub>E # p)" in allE, simp)
+      then have 1: "Y \<inter> {ea. ea \<noteq> Tock \<and> (\<exists>x. (\<exists>p. x = hide_trace X p \<and> p \<in> {\<sigma>. [Event e]\<^sub>E # \<sigma> \<in> P}) \<and> \<rho> @ [[ea]\<^sub>E] \<in> x) \<or>
+              ea = Tock \<and> (\<exists>x. (\<exists>p. x = hide_trace X p \<and> p \<in> {\<sigma>. [Event e]\<^sub>E # \<sigma> \<in> P}) \<and> \<rho> @ [[Xa]\<^sub>R, [ea]\<^sub>E] \<in> x)} = {}"
+        by (smt case_assms(1) disjoint_iff_not_equal subsetCE)
+      have 2: "CT2 {\<sigma>. [Event e]\<^sub>E # \<sigma> \<in> P}"
+        using case_assms(3) unfolding CT2_def by (auto, erule_tac x="[Event e]\<^sub>E # \<rho>" in allE, auto)
+      show "\<exists>x. (\<exists>p. x = hide_trace X p \<and> p \<in> P) \<and> \<rho> @ [[Xa \<union> Y]\<^sub>R] \<in> x"
+        using ind_hyp[where P="{\<sigma>. [Event e]\<^sub>E # \<sigma> \<in> P}", where \<rho>=\<rho>] 1 2 case_assms by auto
+    next
+      fix e \<sigma> P \<rho> s'
+      assume ind_hyp: "\<And>P \<rho>. Y \<inter> {e. e \<noteq> Tock \<and> (\<exists>x. (\<exists>p. x = hide_trace X p \<and> p \<in> P) \<and> \<rho> @ [[e]\<^sub>E] \<in> x) \<or>
+                       e = Tock \<and> (\<exists>x. (\<exists>p. x = hide_trace X p \<and> p \<in> P) \<and> \<rho> @ [[Xa]\<^sub>R, [e]\<^sub>E] \<in> x)} = {} \<Longrightarrow>
+        \<rho> @ [[Xa]\<^sub>R] \<in> hide_trace X \<sigma> \<Longrightarrow> \<sigma> \<in> P \<Longrightarrow> CT2 P \<Longrightarrow> \<exists>x. (\<exists>p. x = hide_trace X p \<and> p \<in> P) \<and> \<rho> @ [[Xa \<union> Y]\<^sub>R] \<in> x"
+      assume case_assms: "Y \<inter> {e. e \<noteq> Tock \<and> (\<exists>x. (\<exists>p. x = hide_trace X p \<and> p \<in> P) \<and> \<rho> @ [[e]\<^sub>E] \<in> x) \<or>
+                e = Tock \<and> (\<exists>x. (\<exists>p. x = hide_trace X p \<and> p \<in> P) \<and> \<rho> @ [[Xa]\<^sub>R, [e]\<^sub>E] \<in> x)} = {}"
+        "[Event e]\<^sub>E # \<sigma> \<in> P" "CT2 P" "Event e \<notin> X" "s' \<in> hide_trace X \<sigma>" "\<rho> @ [[Xa]\<^sub>R] = [Event e]\<^sub>E # s'"
+      then obtain \<rho>' where \<rho>'_assms: "\<rho> = [Event e]\<^sub>E # \<rho>' \<and> \<rho>' @ [[Xa]\<^sub>R] \<in> hide_trace X \<sigma>"
+        by (cases \<rho> rule:cttWF.cases, simp_all, blast)
+      have "{ea. ea \<noteq> Tock \<and> (\<exists>x. (\<exists>p. x = hide_trace X p \<and> p \<in> {\<sigma>. [Event e]\<^sub>E # \<sigma> \<in> P}) \<and> \<rho>' @ [[ea]\<^sub>E] \<in> x) \<or>
+          ea = Tock \<and> (\<exists>x. (\<exists>p. x = hide_trace X p \<and> p \<in> {\<sigma>. [Event e]\<^sub>E # \<sigma> \<in> P}) \<and> \<rho>' @ [[Xa]\<^sub>R, [ea]\<^sub>E] \<in> x)} \<subseteq>
+        {e. e \<noteq> Tock \<and> (\<exists>x. (\<exists>p. x = hide_trace X p \<and> p \<in> P) \<and> \<rho> @ [[e]\<^sub>E] \<in> x) \<or>
+          e = Tock \<and> (\<exists>x. (\<exists>p. x = hide_trace X p \<and> p \<in> P) \<and> \<rho> @ [[Xa]\<^sub>R, [e]\<^sub>E] \<in> x)}"
+        using \<rho>'_assms case_assms(4) by auto
+      then have 1: "Y \<inter> {ea. ea \<noteq> Tock \<and> (\<exists>x. (\<exists>p. x = hide_trace X p \<and> p \<in> {\<sigma>. [Event e]\<^sub>E # \<sigma> \<in> P}) \<and> \<rho>' @ [[ea]\<^sub>E] \<in> x) \<or>
+          ea = Tock \<and> (\<exists>x. (\<exists>p. x = hide_trace X p \<and> p \<in> {\<sigma>. [Event e]\<^sub>E # \<sigma> \<in> P}) \<and> \<rho>' @ [[Xa]\<^sub>R, [ea]\<^sub>E] \<in> x)} = {}"
+        by (smt case_assms(1) disjoint_iff_not_equal subsetCE)
+      have 2: "CT2 {\<sigma>. [Event e]\<^sub>E # \<sigma> \<in> P}"
+        using case_assms(3) unfolding CT2_def by (auto, erule_tac x="[Event e]\<^sub>E # \<rho>" in allE, auto)
+      have "\<exists>x. (\<exists>p. x = hide_trace X p \<and> p \<in> {\<sigma>. [Event e]\<^sub>E # \<sigma> \<in> P}) \<and> \<rho>' @ [[Xa \<union> Y]\<^sub>R] \<in> x"
+        using ind_hyp[where P="{\<sigma>. [Event e]\<^sub>E # \<sigma> \<in> P}", where \<rho>="\<rho>'"] 1 2 \<rho>'_assms case_assms by auto
+      then obtain x p where "x = hide_trace X p \<and> p \<in> {\<sigma>. [Event e]\<^sub>E # \<sigma> \<in> P} \<and> \<rho>' @ [[Xa \<union> Y]\<^sub>R] \<in> x"
+        by auto
+      then show "\<exists>x. (\<exists>p. x = hide_trace X p \<and> p \<in> P) \<and> \<rho> @ [[Xa \<union> Y]\<^sub>R] \<in> x"
+        using case_assms \<rho>'_assms by (rule_tac x="hide_trace X ([Event e]\<^sub>E # p)" in exI, auto)
+    next
+      fix Xb \<sigma> P \<rho>
+      assume ind_hyp: "\<And>P \<rho>. Y \<inter> {e. e \<noteq> Tock \<and> (\<exists>x. (\<exists>p. x = hide_trace X p \<and> p \<in> P) \<and> \<rho> @ [[e]\<^sub>E] \<in> x) \<or>
+                       e = Tock \<and> (\<exists>x. (\<exists>p. x = hide_trace X p \<and> p \<in> P) \<and> \<rho> @ [[Xa]\<^sub>R, [e]\<^sub>E] \<in> x)} = {} \<Longrightarrow>
+        \<rho> @ [[Xa]\<^sub>R] \<in> hide_trace X \<sigma> \<Longrightarrow> \<sigma> \<in> P \<Longrightarrow> CT2 P \<Longrightarrow> \<exists>x. (\<exists>p. x = hide_trace X p \<and> p \<in> P) \<and> \<rho> @ [[Xa \<union> Y]\<^sub>R] \<in> x"
+      assume case_assms: "Y \<inter> {e. e \<noteq> Tock \<and> (\<exists>x. (\<exists>p. x = hide_trace X p \<and> p \<in> P) \<and> \<rho> @ [[e]\<^sub>E] \<in> x) \<or>
+                e = Tock \<and> (\<exists>x. (\<exists>p. x = hide_trace X p \<and> p \<in> P) \<and> \<rho> @ [[Xa]\<^sub>R, [e]\<^sub>E] \<in> x)} = {}"
+        "[Xb]\<^sub>R # [Tock]\<^sub>E # \<sigma> \<in> P" "CT2 P" "Tock \<in> X" "\<rho> @ [[Xa]\<^sub>R] \<in> hide_trace X \<sigma>"
+      have "{e. e \<noteq> Tock \<and> (\<exists>x. (\<exists>p. x = hide_trace X p \<and> p \<in> {\<sigma>. [Xb]\<^sub>R # [Tock]\<^sub>E # \<sigma> \<in> P}) \<and> \<rho> @ [[e]\<^sub>E] \<in> x) \<or>
+          e = Tock \<and> (\<exists>x. (\<exists>p. x = hide_trace X p \<and> p \<in> {\<sigma>. [Xb]\<^sub>R # [Tock]\<^sub>E # \<sigma> \<in> P}) \<and> \<rho> @ [[Xa]\<^sub>R, [e]\<^sub>E] \<in> x)} \<subseteq>
+        {e. e \<noteq> Tock \<and> (\<exists>x. (\<exists>p. x = hide_trace X p \<and> p \<in> P) \<and> \<rho> @ [[e]\<^sub>E] \<in> x) \<or>
+          e = Tock \<and> (\<exists>x. (\<exists>p. x = hide_trace X p \<and> p \<in> P) \<and> \<rho> @ [[Xa]\<^sub>R, [e]\<^sub>E] \<in> x)}"
+        using case_assms(2) case_assms(4) case_assms(5) by (auto)
+      then have 1: "Y \<inter> {e. e \<noteq> Tock \<and> (\<exists>x. (\<exists>p. x = hide_trace X p \<and> p \<in> {\<sigma>. [Xb]\<^sub>R # [Tock]\<^sub>E # \<sigma> \<in> P}) \<and> \<rho> @ [[e]\<^sub>E] \<in> x) \<or>
+          e = Tock \<and> (\<exists>x. (\<exists>p. x = hide_trace X p \<and> p \<in> {\<sigma>. [Xb]\<^sub>R # [Tock]\<^sub>E # \<sigma> \<in> P}) \<and> \<rho> @ [[Xa]\<^sub>R, [e]\<^sub>E] \<in> x)} = {}"
+        by (smt case_assms(1) disjoint_iff_not_equal subsetCE)
+      have 2: "CT2 {\<sigma>. [Xb]\<^sub>R # [Tock]\<^sub>E # \<sigma> \<in> P}"
+        using case_assms(3) unfolding CT2_def by (auto, erule_tac x="[Xb]\<^sub>R # [Tock]\<^sub>E # \<rho>" in allE, auto)
+      have "\<exists>x. (\<exists>p. x = hide_trace X p \<and> p \<in> {\<sigma>. [Xb]\<^sub>R # [Tock]\<^sub>E # \<sigma> \<in> P}) \<and> \<rho> @ [[Xa \<union> Y]\<^sub>R] \<in> x"
+        using ind_hyp[where P="{\<sigma>. [Xb]\<^sub>R # [Tock]\<^sub>E # \<sigma> \<in> P}", where \<rho>=\<rho>] 1 2 case_assms by auto
+      then obtain x p where "x = hide_trace X p \<and> p \<in> {\<sigma>. [Xb]\<^sub>R # [Tock]\<^sub>E # \<sigma> \<in> P} \<and> \<rho> @ [[Xa \<union> Y]\<^sub>R] \<in> x"
+        by auto
+      then show "\<exists>x. (\<exists>p. x = hide_trace X p \<and> p \<in> P) \<and> \<rho> @ [[Xa \<union> Y]\<^sub>R] \<in> x"
+        using case_assms by (rule_tac x="hide_trace X ([Xb]\<^sub>R # [Tock]\<^sub>E # p)" in exI, simp, rule_tac x="[Xb]\<^sub>R # [Tock]\<^sub>E # p" in exI, simp)
+    next
+      fix Xb \<sigma> P \<rho> s' Z
+      assume ind_hyp: "\<And>P \<rho>. Y \<inter> {e. e \<noteq> Tock \<and> (\<exists>x. (\<exists>p. x = hide_trace X p \<and> p \<in> P) \<and> \<rho> @ [[e]\<^sub>E] \<in> x) \<or>
+                       e = Tock \<and> (\<exists>x. (\<exists>p. x = hide_trace X p \<and> p \<in> P) \<and> \<rho> @ [[Xa]\<^sub>R, [e]\<^sub>E] \<in> x)} = {} \<Longrightarrow>
+        \<rho> @ [[Xa]\<^sub>R] \<in> hide_trace X \<sigma> \<Longrightarrow> \<sigma> \<in> P \<Longrightarrow> CT2 P \<Longrightarrow> \<exists>x. (\<exists>p. x = hide_trace X p \<and> p \<in> P) \<and> \<rho> @ [[Xa \<union> Y]\<^sub>R] \<in> x"
+      assume case_assms: "Y \<inter> {e. e \<noteq> Tock \<and> (\<exists>x. (\<exists>p. x = hide_trace X p \<and> p \<in> P) \<and> \<rho> @ [[e]\<^sub>E] \<in> x) \<or>
+                e = Tock \<and> (\<exists>x. (\<exists>p. x = hide_trace X p \<and> p \<in> P) \<and> \<rho> @ [[Xa]\<^sub>R, [e]\<^sub>E] \<in> x)} = {}"
+        "[Xb]\<^sub>R # [Tock]\<^sub>E # \<sigma> \<in> P" "CT2 P" "Z \<subseteq> Xb" "Tock \<notin> X" "X \<subseteq> Xb" "\<rho> @ [[Xa]\<^sub>R] = [Z]\<^sub>R # [Tock]\<^sub>E # s'" "s' \<in> hide_trace X \<sigma>"
+      then obtain \<rho>' where \<rho>'_assms: "\<rho> = [Z]\<^sub>R # [Tock]\<^sub>E # \<rho>' \<and> \<rho>' @ [[Xa]\<^sub>R] \<in> hide_trace X \<sigma>"
+        by (cases \<rho> rule:cttWF.cases, simp_all, blast)
+      have "{e. e \<noteq> Tock \<and> (\<exists>x. (\<exists>p. x = hide_trace X p \<and> p \<in> {\<sigma>. [Xb]\<^sub>R # [Tock]\<^sub>E # \<sigma> \<in> P}) \<and> \<rho>' @ [[e]\<^sub>E] \<in> x) \<or>
+          e = Tock \<and> (\<exists>x. (\<exists>p. x = hide_trace X p \<and> p \<in> {\<sigma>. [Xb]\<^sub>R # [Tock]\<^sub>E # \<sigma> \<in> P}) \<and> \<rho>' @ [[Xa]\<^sub>R, [e]\<^sub>E] \<in> x)} \<subseteq>
+        {e. e \<noteq> Tock \<and> (\<exists>x. (\<exists>p. x = hide_trace X p \<and> p \<in> P) \<and> \<rho> @ [[e]\<^sub>E] \<in> x) \<or>
+          e = Tock \<and> (\<exists>x. (\<exists>p. x = hide_trace X p \<and> p \<in> P) \<and> \<rho> @ [[Xa]\<^sub>R, [e]\<^sub>E] \<in> x)}"
+        using case_assms \<rho>'_assms apply (safe, simp_all)
+        apply (rule_tac x="hide_trace X ([Xb]\<^sub>R # [Tock]\<^sub>E # p)" in exI, simp, safe, rule_tac x="[Xb]\<^sub>R # [Tock]\<^sub>E # p" in exI, simp)
+        apply (rule_tac x="hide_trace X ([Xb]\<^sub>R # [Tock]\<^sub>E # p)" in exI, simp, rule_tac x="[Xb]\<^sub>R # [Tock]\<^sub>E # p" in exI, simp)
+        apply (erule_tac x="hide_trace X ([Xb]\<^sub>R # [Tock]\<^sub>E # p)" in allE, simp)
+        by (erule_tac x="hide_trace X ([Xb]\<^sub>R # [Tock]\<^sub>E # p)" in allE, simp)
+      then have 1: "Y \<inter> {e. e \<noteq> Tock \<and> (\<exists>x. (\<exists>p. x = hide_trace X p \<and> p \<in> {\<sigma>. [Xb]\<^sub>R # [Tock]\<^sub>E # \<sigma> \<in> P}) \<and> \<rho>' @ [[e]\<^sub>E] \<in> x) \<or>
+          e = Tock \<and> (\<exists>x. (\<exists>p. x = hide_trace X p \<and> p \<in> {\<sigma>. [Xb]\<^sub>R # [Tock]\<^sub>E # \<sigma> \<in> P}) \<and> \<rho>' @ [[Xa]\<^sub>R, [e]\<^sub>E] \<in> x)} = {}"
+        by (smt case_assms(1) disjoint_iff_not_equal subsetCE)
+      have 2: "CT2 {\<sigma>. [Xb]\<^sub>R # [Tock]\<^sub>E # \<sigma> \<in> P}"
+        using case_assms(3) unfolding CT2_def by (auto, erule_tac x="[Xb]\<^sub>R # [Tock]\<^sub>E # \<rho>" in allE, auto)
+      have "\<exists>x. (\<exists>p. x = hide_trace X p \<and> p \<in> {\<sigma>. [Xb]\<^sub>R # [Tock]\<^sub>E # \<sigma> \<in> P}) \<and> \<rho>' @ [[Xa \<union> Y]\<^sub>R] \<in> x"
+        using ind_hyp[where P="{\<sigma>. [Xb]\<^sub>R # [Tock]\<^sub>E # \<sigma> \<in> P}", where \<rho>=\<rho>'] 1 2 case_assms \<rho>'_assms by auto
+      then obtain x p where "x = hide_trace X p \<and> p \<in> {\<sigma>. [Xb]\<^sub>R # [Tock]\<^sub>E # \<sigma> \<in> P} \<and> \<rho>' @ [[Xa \<union> Y]\<^sub>R] \<in> x"
+        by auto
+      then show "\<exists>x. (\<exists>p. x = hide_trace X p \<and> p \<in> P) \<and> \<rho> @ [[Xa \<union> Y]\<^sub>R] \<in> x"
+        using case_assms \<rho>'_assms by (rule_tac x="hide_trace X ([Xb]\<^sub>R # [Tock]\<^sub>E # p)" in exI, auto)
+    qed
+  qed
+qed
